src/Dep.v
@@ -1,0 +1,172 @@
+Require Import Coq.Structures.OrderedType.
+Require Import Coq.Structures.OrderedTypeEx.
+Require Import Coq.FSets.FMapAVL.
+Require Import Coq.FSets.FSetAVL.
+Require Import Coq.Arith.Peano_dec.
+Require Import Aniceto.Map.
+
+Require Coq.FSets.FMapFacts.
+
+Require Import HJ.Mid.
+Require Import HJ.Tid.
+
+Notation dep := (mid + tid)%type.
+
+Notation d_mid := (@inl mid tid).
+
+Notation d_tid := (@inr mid tid).
+
+Module SumOrderedType (O1 O2:OrderedType) <: OrderedType.
+  Definition t := sum O1.t O2.t.
+  Definition eq o1 o2 :=
+    match o1 with
+    | inl l =>
+      match o2 with
+      | inl r => O1.eq l r
+      | inr r => False
+      end
+    | inr l =>
+      match o2 with
+      | inl r => False
+      | inr r => O2.eq l r
+      end
+    end.
+    
+  Definition lt o1 o2 :=
+    match o1 with
+    | inl l =>
+      match o2 with
+      | inl r => O1.lt l r
+      | inr r => True
+      end
+    | inr l =>
+      match o2 with
+      | inl r => False
+      | inr r => O2.lt l r
+      end
+    end.
+
+  Lemma eq_refl:
+    forall x,
+    eq x x.
+  Proof.
+    intros.
+    destruct x; simpl; eauto using O1.eq_refl, O2.eq_refl.
+  Qed.
+
+  Lemma eq_sym:
+    forall x y,
+    eq x y ->
+    eq y x.
+  Proof.
+    intros.
+    destruct x, y; simpl in *; eauto using O1.eq_sym, O2.eq_sym.
+  Qed.
+
+  Lemma eq_trans :
+    forall x y z,
+    eq x y ->
+    eq y z ->
+    eq x z.
+  Proof.
+    intros.
+    destruct x, y, z; simpl in *.
+    - eauto using O1.eq_trans.
+    - inversion H0.
+    - inversion H0.
+    - inversion H.
+    - inversion H.
+    - inversion H.
+    - inversion H0.
+    - eauto using O2.eq_trans.
+  Qed.
+
+  Lemma lt_trans:
+    forall x y z : t, lt x y -> lt y z -> lt x z.
+  Proof.
+    intros.
+    unfold lt in *.
+    destruct x, y, z; auto.
+    - eauto using O1.lt_trans.
+    - inversion H0.
+    - inversion H.
+    - eauto using O2.lt_trans.
+  Qed.
+
+  Lemma lt_not_eq : forall x y : t, lt x y -> ~ eq x y.
+  Proof.
+    intros.
+    destruct x, y; simpl in *.
+    - eauto using O1.lt_not_eq.
+    - intuition; inversion H0.
+    - inversion H.
+    - eauto using O2.lt_not_eq.
+  Qed.
+
+  Require Import Coq.Arith.Compare_dec.
+  Lemma compare:
+    forall x y, Compare lt eq x y.
+  Proof.
+    intros.
+    destruct x, y.
+    - assert (C: Compare O1.lt O1.eq t0 t1) by eauto using O1.compare.
+      destruct C; eauto using LT, EQ, GT.
+    - apply LT.
+      simpl.
+      trivial.
+    - apply GT.
+      simpl.
+      trivial.
+    - assert (C: Compare O2.lt O2.eq t0 t1) by eauto using O2.compare.
+      destruct C; eauto using LT, EQ, GT.
+  Qed.
+
+  Lemma eq_dec : forall x y : t, {eq x y} + {~ eq x y}.
+  Proof.
+    intros.
+    destruct x, y; simpl; eauto using O1.eq_dec, O2.eq_dec.
+  Qed.
+
+  Lemma eq_rw
+    (o1_eq_rw: forall x y, O1.eq x y <-> x = y)
+    (o2_eq_rw: forall x y, O2.eq x y <-> x = y):
+    forall x y, eq x y <-> x = y.
+  Proof.
+    intros.
+    destruct x, y; simpl in *.
+    - split.
+      + intros.
+        apply o1_eq_rw in H; subst.
+        trivial.
+      + intros.
+        inversion H; subst.
+        rewrite o1_eq_rw.
+        trivial.
+    - split; intros; inversion H.
+    - split; intros; inversion H.
+    - split.
+      + intros.
+        apply o2_eq_rw in H; subst.
+        trivial.
+      + intros.
+        inversion H; subst.
+        rewrite o2_eq_rw.
+        trivial.
+  Qed.
+
+End SumOrderedType.
+
+Module DEP := SumOrderedType MID TID.
+
+Lemma dep_eq_rw:
+  forall x y, DEP.eq x y <-> x = y.
+Proof.
+  intros.
+  split;
+  intros;
+  apply DEP.eq_rw in H; auto using mid_eq_rw, tid_eq_rw.
+Qed.
+
+Module SD := FSetAVL.Make DEP.
+Definition set_dep := SD.t.
+
